test/ctypes/Lowlevel.fst
@@ -8,10 +8,11 @@ module B = LowStar.Buffer
 module M = LowStar.Modifies
 module U32 = FStar.UInt32
 
-type point = { x: UInt32.t; y: UInt32.t }
-type circle = { c: point; r: UInt32.t}
+type point = { x: U32.t; y: U32.t }
+type circle = { c: point; r: U32.t }
 
-let square (x: UInt32.t): UInt32.t =
+let square (x: U32.t): U32.t =
+
   let open FStar.UInt32 in
   x *%^ x
 
@@ -33,3 +34,60 @@ val move_circle: cir: circle -> d: point -> Stack circle
 let move_circle cir d =
   let open FStar.UInt32 in
   { cir with c = point_sum cir.c d }
+
+// Inductives: enum compilation scheme
+type my_bool = | MyTrue | MyFalse
+val my_not: b: B.pointer my_bool -> Stack unit
+  (requires fun h -> B.live h b)
+  (requires fun h0 _ h1 -> True)
+let my_not b =
+  let open LowStar.Monotonic.Buffer in
+  let v = match B.index b 0ul with
+    | MyTrue -> MyFalse
+    | MyFalse -> MyTrue
+  in
+  upd b 0ul v;
+  ()
+
+// Inductives: record compilation scheme
+type tr = | Rec of U32.t * U32.t * U32.t * U32.t * U32.t
+val replicate: n: U32.t -> Stack tr
+  (requires fun h -> True)
+  (requires fun h0 _ h1 -> True)
+let replicate n =
+  Rec (n, n, n, n, n)
+
+
+// // Inductives: optimised flat compilation scheme
+// type int_opt = | Some of U32.t | None
+
+// // Inductives: general compilation scheme
+// assume new type foo
+// assume new type bar
+// noeq type t_general = | A of foo | B of bar
+
+
+// val my_not: b: B.pointer U32.t -> Stack unit
+//   (requires fun h -> B.live h b)
+//   (requires fun h0 _ h1 -> B.live h1 b)
+// let my_not b =
+//   let open LowStar.Monotonic.Buffer in
+//   let v = B.index b 0ul in
+//   upd b 0ul 5ul;
+//   ()
+
+
+// val new_buf: last: U32.t -> Stack (FStar.Seq.lseq U32.t 5 )
+//   (requires fun h -> True)
+//   (requires fun h0 _ h1 -> True)
+// let new_buf last =
+//   FStar.Seq.createL [1ul; 2ul; 3ul; 4ul; last]
+
+
+// val list_of_circles: cir: circle -> n: U32.t -> Stack circle
+//   (requires fun h ->
+//     U32.v cir.c.x + U32.v d.x < 32 /\
+//     U32.v cir.c.y + U32.v d.y < 32)
+//   (requires fun h0 _ h1 -> True)
+// let rec list_of_circles cir n =
+  
